Detect and prune rewrites with unsynthesizable type class conditions
This is useful when using explosion, as it can generate rewrites with bogus conditions

Lean/Egg/Tests/Class Def.lean
@@ -1,14 +1,14 @@
 import Egg
 
-def Mul.pow [Mul α] [OfNat α 1] (a : α) : Nat → α
+def Mul.pow [Mul α] [One α] (a : α) : Nat → α
   | 0     => 1
   | n + 1 => a * (pow a n)
 
-instance mulPow [Mul α] [OfNat α 1] : Pow α Nat where
+instance mulPow [Mul α] [One α] : Pow α Nat where
   pow := Mul.pow
 
-example [Mul α] [OfNat α 1] (a : α) : Mul.pow a 0 = (1 : α) := by
+example [Mul α] [One α] (a : α) : Mul.pow a 0 = (1 : α) := by
   egg [Mul.pow]
 
-example [Mul α] [OfNat α 1] (a : α) : a ^ 0 = (1 : α) := by
+example [Mul α] [One α] (a : α) : a ^ 0 = (1 : α) := by
   egg [Mul.pow]
