Lean/Egg/Tests/Shapes.lean
@@ -101,24 +101,22 @@ end Binders
 
 section «Class Def»
 
-def Mul.pow [Mul α] [OfNat α 1] (a : α) : Nat → α
+def Mul.pow [Mul α] [One α] (a : α) : Nat → α
   | 0     => 1
   | n + 1 => a * (pow a n)
 
-instance mulPow [Mul α] [OfNat α 1] : Pow α Nat where
+instance mulPow [Mul α] [One α] : Pow α Nat where
   pow := Mul.pow
 
-example [Mul α] [OfNat α 1] (a : α) : Mul.pow a 0 = (1 : α) := by
+example [Mul α] [One α] (a : α) : Mul.pow a 0 = (1 : α) := by
   egg [Mul.pow]
 
-example [Mul α] [OfNat α 1] (a : α) : a ^ 0 = (1 : α) := by
+example [Mul α] [One α] (a : α) : a ^ 0 = (1 : α) := by
   egg [Mul.pow]
 
 end «Class Def»
 
 section Groups
-
-instance [One α] : OfNat α 1 where ofNat := One.one
 
 class Group (α) extends One α, Inv α, Mul α where
   mul_assoc     (a b c : α) : (a * b) * c = a * (b * c)
