Lean/Egg/Core/Gen/Explosion.lean
@@ -26,32 +26,29 @@ private partial def exprReferencesMVar (e : Expr) (m : MVarId) : MetaM Bool := d
 private partial def genExplosionsForRw (rw : Rewrite) (subgoals : Bool) : MetaM Rewrites := do
   let mut missing := rw.mvars.rhs.visibleExpr.subtract rw.mvars.lhs.visibleExpr
   for violation in ← rw.violations subgoals do
-    let .lhsSingleMVar m := violation | continue
-    missing := missing.insert m
-  return (← genDir .forward missing)
+    if let .lhsSingleMVar m := violation then
+      missing := missing.insert m
+      break
+  if missing.isEmpty then return #[]
+  let ordered ← missing.toList.qsortM fun m₁ m₂ => return !(← exprReferencesMVar (.mvar m₁) m₂)
+  core rw ordered []
 where
-  genDir (dir : Direction) (missing : MVarIdSet) : MetaM Rewrites := do
-    if missing.isEmpty then return #[]
-    let ordered ← missing.toList.qsortM fun m₁ m₂ => return !(← exprReferencesMVar (.mvar m₁) m₂)
-    core rw dir ordered []
-  core (rw : Rewrite) (dir : Direction) (missing : List MVarId) (loc : List Nat) :
-      MetaM Rewrites := do
-    let m :: miss := missing | return #[← rw.fresh (src := .explosion rw.src dir loc)]
-    let lctx ← getLCtx
+  core (rw : Rewrite) (missing : List MVarId) (loc : List Nat) : MetaM Rewrites := do
+    let m :: miss := missing | return #[← rw.fresh (src := .explosion rw.src loc)]
     let mut minIdx := 0
     let mut explosions : Rewrites := #[]
-    while minIdx < lctx.decls.size do
+    while minIdx < (← getLCtx).decls.size do
       let (fresh, subst) ← rw.freshWithSubst
       let m := subst.expr[m]!
       let some (fvar, idx) ← findLocalDeclWithTypeMinIdx? (← m.getType) minIdx | break
       minIdx := idx + 1
-      -- TODO: Only have this succeed when type correct.
       unless ← isDefEq (.mvar m) (.fvar fvar) do throwError "egg: internal error in explosion gen"
       let fresh ← fresh.instantiateMVars
+      unless fresh.conds.unsynthesizable.isEmpty do continue
       let miss := miss.filterMap fun i =>
         let i' := subst.expr[i]!
         if fresh.mvars.lhs.expr.contains i' || fresh.mvars.rhs.expr.contains i' then i' else none
-      explosions := explosions ++ (← core fresh dir miss <| loc ++ [minIdx])
+      explosions := explosions ++ (← core fresh miss <| loc ++ [minIdx])
     return explosions
 
 def genExplosions (targets : Rewrites) (subgoals : Bool) : MetaM Rewrites := do
