Lean/Egg/Core/Rewrite/Condition.lean
@@ -32,6 +32,7 @@ structure _root_.Egg.Rewrite.Condition where
 inductive Result where
   | none
   | synthesized
+  | unsynthesizable
   | some (cond : Condition)
 
 def from? (mvar : MVarId) (lhs : MVars) : MetaM Result := do
@@ -40,9 +41,10 @@ def from? (mvar : MVarId) (lhs : MVars) : MetaM Result := do
   let type ← instantiateMVars (← inferType <| .mvar mvar)
   -- This is a small optimization. If a type class can already be synthesized, we do it immediately
   -- and don't generate a condition to be synthesized during eqsat.
-  if ← trySynthesizeTcInst type kind
-  then return .synthesized
-  else return .some { kind, mvar, type }
+  match ← trySynthesizeTcInst type kind with
+  | .undef => return .some { kind, mvar, type }
+  | .true  => return .synthesized
+  | .false => return .unsynthesizable
 where
   -- If the mvar appears in the LHS, then it's a condition only if it's a nested instance or proof.
   -- If it does not appear in the LHS, it's a condition immediately if it's an instance or proof.
@@ -57,14 +59,14 @@ where
     else if ← isProof (.mvar mvar) then
       return some .proof
     return none
-  trySynthesizeTcInst (type : Expr) : Kind → MetaM Bool
-  | .proof  => return false
+  trySynthesizeTcInst (type : Expr) : Kind → MetaM LBool
+  | .proof  => return .undef
   | .tcInst => do
-    if type.hasMVar then return false
-    let some inst ← synthInstance? type | return false
+    if type.hasMVar then return .undef
+    let some inst ← synthInstance? type | return .false
     unless ← isDefEq (.mvar mvar) inst do
       throwError "Internal error in 'Egg.Rewrite.Condition.from?.synthesizeTcInst?'"
-    return true
+    return .true
 
 def fresh (cond : Condition) (init : MVars.Subst) : MetaM (Condition × MVars.Subst) := do
   let (_, subst) ← (← MVars.collect <| .mvar cond.mvar).fresh init
